imp/Imp/Hoare/Basic.lean
@@ -1,0 +1,49 @@
+import Imp.Expr.Eval
+import Imp.Stmt.BigStep
+import Imp.Stmt.Basic
+
+open Imp Stmt
+
+@[simp]
+def ValidHoareTriple (P : Env → Prop) (c : Stmt) (Q : Env → Prop) : Prop :=
+  forall (st st' : Env), P st -> c / st ↓ st' -> Q st'
+
+syntax "{{" term:90 "}} " term:91 " {{" term:92 "}}" : term
+macro_rules
+  | `({{$P}}$c{{$Q}}) => `(ValidHoareTriple $P $c $Q)
+
+theorem hoare_skip : forall P, {{P}}(imp { skip; }){{P}} := by
+  intro P
+  simp [ValidHoareTriple]
+  intros st st' h1 h2
+  cases h2; assumption
+
+theorem hoare_seq : forall P Q R c1 c2, {{P}}c1{{Q}} -> {{Q}}c2{{R}} -> {{P}}(imp { ~c1 ~c2 }){{R}} := by
+  intro P Q R c1 c2
+  simp [ValidHoareTriple]
+  intros h1 h2 st st' hP h3
+  cases h3 with
+  | seq h3 h4 =>
+    apply h2
+    apply h1
+    apply hP
+    apply h3
+    apply h4
+
+def assertionSubstitution (P : Env → Prop) (x : String) (a : Expr) : Env → Prop :=
+  fun st => P (st.setOption x (Expr.eval st a))
+
+syntax term " [ " ident " |-> " term "]" : term
+macro_rules
+  | `($P [$x |-> $a]) => `(assertionSubstitution $P $x $a)
+
+theorem hoare_assign : forall P x a, {{P[x |-> a]}}(imp { ~x := a; }){{P}} := by
+  intros P x a
+  simp [ValidHoareTriple]
+  intros st st' h1 h2
+  cases h2 with
+  | assign h3 =>
+    simp [assertionSubstitution] at h1
+    simp [Expr.eval, Env.get] at h3
+    simp [Env.setOption] at h1
+    sorry
