README.md
@@ -1,1 +1,36 @@
 # Formally Verified APPS
+
+## Conceptually 1
+- llm-solve an apps subset in imp, at least in slow versions
+- Provided in benchmark:
+  - write slow imp programs
+  - write hoare triples
+  - prove hoare triples
+- Task;
+  - ask llm to write faster versions
+  - proof of hoare agreement
+
+### value prop
+- challenging LLMs to write formally verified code.
+
+### TODO
+- [ ] some array story in Imp
+- [ ] strings in imp?
+
+## Conceptually 2
+- find two implementations of the same problem
+- quantify over all inputs that they agree
+
+### Question
+- mathlib free or mathlib
+
+### Value prop
+challenging LLMs to write dependently typed _and_ formally verified code
+
+### TODO
+- [ ] trawl aoc of the ones we have lean4 solutions for some nontriviality:
+  - meaning a way to beat the dumb way on O()
+
+## TODO
+- [ ] read dafny benchmark paper
+- [ ] read the APPS easies.
